\documentclass[aps,12pt]{revtex4}
\usepackage{graphicx}
\usepackage{amssymb,amsfonts,amsmath,amsthm}
\usepackage{chemarr}
\usepackage{bm}
\usepackage{pslatex}
\usepackage{bookman}



\begin{document}
\title{Arcs}
\maketitle
	
\section{Definitions}

\subsection{Positions}
We have a set of $N$ points $\vec{P}_1,\ldots,\vec{P}_N$, each point in $\mathbb{R}^d$ (where $d$ is the space dimension), and we assume
that they describe a virtual arc for a dimensionless coordinate $t_i=i$.

\subsection{Velocities}

\subsubsection{Bulk Case}

\begin{equation}
	\forall 1<i<N,
	\left\lbrace
	\begin{array}{rcl}
	\vec{V}_i & = & \frac{1}{2}\left(\vec{P}_{i+1} - \vec{P}_{i-1}\right)\\
	\vec{A}_i & = &  \vec{P}_{i+1} - \vec{P}_{i-1} + 2\vec{P}_i\\
	\end{array}
	\right.
\end{equation}

\subsubsection{Standard Case Boundaries}
\begin{equation}
\begin{array}{rl}
N=2 &
	\left\lbrace
	\begin{array}{rcl}
	\vec{V}_1 & = &  \left( \vec{P}_2 - \vec{P}_1\right)\\
	\vec{V}_2 & = &  \left( \vec{P}_2 - \vec{P}_1\right) = \vec{V}_1\\
	\vec{A}_1 & = & \vec{0}\\
	\vec{A}_2 & = & \vec{0}\\
	\end{array}
	\right.
	\\
	\\
	N\geq3 & 
	\left\lbrace
	\begin{array}{rcl}
	\vec{V}_1 & = & \frac{1}{2} \left[ 4\vec{P}_2     - (3\vec{P}_1+\vec{P}_3)\right]\\
	\vec{V}_N & = & \frac{1}{2} \left[ (3\vec{P}_{N}+\vec{P}_{N-2})-4\vec{P}_{N-1} \right]\\
	\vec{A}_1 & = & \vec{P}_3+\vec{P}_1-2\vec{P}_2         \\
	\vec{A}_N & = & \vec{P}_N+\vec{P}_{N-2}-2\vec{P}_{N-1} \\
	\end{array}
	\right.
\end{array}
\end{equation}

 
\subsubsection{Periodic Case Boundaries}

\begin{equation}
\begin{array}{rl}
N=2 &
	\left\lbrace
	\begin{array}{rcl}
	\vec{V}_1 & = &  \left( \vec{P}_2 - \vec{P}_1\right)\\
	\vec{V}_2 & = &  \left( \vec{P}_1 - \vec{P}_2\right) = -\vec{V}_1\\
	\vec{A}_1 & = & \vec{0}\\
	\vec{A}_2 & = & \vec{0}\\
	\end{array}
	\right.
	\\
	\\
	N\geq3 & 
	\left\lbrace
	\begin{array}{rcl}
	\vec{V}_1 & = & \frac{1}{2} \left( \vec{P}_2 - \vec{P}_N\right)\\
	\vec{V}_N & = & \frac{1}{2} \left( \vec{P}_1 - \vec{P}_{N-1}\right)\\
	\vec{A}_1 & = & \vec{P}_2+\vec{P}_{N}-2\vec{P}_1         \\
	\vec{A}_N & = & \vec{P}_1+\vec{P}_{N-1}-2\vec{P}_{N} \\
	\end{array}
	\right.
\end{array}
\end{equation}

\subsection{Generic Index}
We define:
\begin{equation}
	i' =
	\left\lbrace
	\begin{array}{rcl}
		i+1 & \mbox{if } i<N\\
		1   & \mbox{if } i=N\\
	\end{array}
	\right.
\end{equation}


\section{Arcs}

\subsection{$\mathcal{C}^0$ Arcs}

\begin{equation}
	\vec{P}(u) = \vec{P}_i + u \left(\vec{P}_{i'} - \vec{P}_{i}\right)
\end{equation}

\subsection{$\mathcal{C}^1$ Arcs}

\begin{equation}
	\vec{V}(t) = \vec{V}_i + t \left(\vec{V}_{i'}-\vec{V}_i\right) + t(1-t) \vec{Q}_i
\end{equation}

\begin{equation}
	\vec{P}(t) = \vec{P}_i + \int_0^t \vec{V}(u) \, \mathrm{d} u 
	= \vec{P}_i + t\vec{V}_i  + \frac{t^2}{2} \left(\vec{V}_{i'}-\vec{V}_i\right) + \left(\frac{t^2}{2} - \frac{t^3}{3}\right) \vec{Q}_i
\end{equation}

\begin{equation}
	\vec{P}_i' = \vec{P}_i + \vec{V}_i  + \frac{1}{2} \left(\vec{V}_{i'}-\vec{V}_i\right) + \frac{1}{6} \vec{Q}_i
\end{equation}


\begin{equation}
	\boxed{\vec{Q}_i = 6\left(\vec{P}_i'-\vec{P}_i\right) - 3  \left(\vec{V}_{i'}+\vec{V}_i\right)}
\end{equation}


\subsection{$\mathcal{C}^2$ Arcs}

\begin{equation}
	\vec{A}(t) = \vec{A}_i + t\left(\vec{A}_{i'}-\vec{A}_{i}\right) + t(1-t)(\vec{Q}_i+t\vec{W}_i)
\end{equation}

\begin{equation}
	\vec{V}(t) =  \vec{V}_i + \int_0^t \vec{A}(u) \, \mathrm{d} u 
	= \vec{V}_i + t \vec{A}_i + \frac{t^2}{2} \left(\vec{A}_{i'}-\vec{A}_{i}\right) 
	+ \left(\frac{t^2}{2} - \frac{t^3}{3}\right)  \vec{Q}_i 
	+ \left(\frac{t^3}{3} - \frac{t^4}{4}\right)  \vec{W}_i
	\end{equation}

\begin{equation}
\label{eq:v}
\boxed{
	\vec{V}_{i'} = \vec{V}_i + \frac{1}{2} \left( \vec{A}_{i}+\vec{A}_{i'}\right) + \frac{1}{6}\vec{Q}_i + \frac{1}{12}\vec{W}_i
	}
\end{equation}

\begin{equation}
\begin{array}{rcl}
	\vec{P}(t) &=& \displaystyle \vec{P}_i + \int_0^t \vec{V}(u) \, \mathrm{d} u \\
	\\
	& = & \displaystyle \vec{P}_i + t \vec{V}_i + \frac{t^2}{2} \vec{A}_i + \frac{t^3}{6}  \left(\vec{A}_{i'}-\vec{A}_{i}\right) 
	+ \left(\frac{t^3}{6} - \frac{t^4}{12}\right)  \vec{Q}_i +  \left(\frac{t^4}{12} - \frac{t^5}{20}\right) \vec{W}_i\\
\end{array}
\end{equation}

\begin{equation}
	\vec{P}_{i'} = \vec{P}_i + \vec{V}_i + \frac{1}{2} \vec{A}_i + \frac{1}{6} \left(\vec{A}_{i'}-\vec{A}_{i}\right) + \frac{1}{12} \vec{Q}_i + \frac{1}{30} \vec{W}_i
\end{equation}

\begin{equation}
\label{eq:p}
\boxed{
	\vec{P}_{i'} = \vec{P}_i + \vec{V}_i + \frac{1}{3} \vec{A}_i + \frac{1}{6}  \vec{A}_{i'}  + \frac{1}{12} \vec{Q}_i + \frac{1}{30} \vec{W}_i
	}
\end{equation}

\begin{equation}
\begin{array}{rcl}
	\vec{Q}_i & = & 60\left(\vec{P}_{i'}-\vec{P}_i\right) - 6\left(6\vec{V}_i+4\vec{V}_{i'}\right) - 2 \left(4\vec{A}_{i}-\vec{A}_{i'}\right)  \\
	\vec{W}_i & = & 60\left(\vec{V}_i+\vec{V}_{i'}\right) - 120 \left(\vec{P}_{i'}-\vec{P}_i\right) -10\left(\vec{A}_{i'} - \vec{A}_{i}\right) \\
\end{array}
\end{equation}


\end{document}



