\documentclass[aps,12pt]{revtex4}
\usepackage{graphicx}
\usepackage{amssymb,amsfonts,amsmath,amsthm}
\usepackage{chemarr}
\usepackage{bm}
\usepackage{pslatex}
\usepackage{mathptmx}
\usepackage{xfrac}
\usepackage{bookman}

%%  
\newcommand{\trn}[1]{{#1}^{\mathtt{t}}}
 
\begin{document}

Let us assume that $\vec{F}(\vec{X})$ is derivable at $\vec{X}$.
Since:
\begin{equation}
	\vec{F}(\vec{X}+\delta\vec{X}) \simeq \vec{F}_0 + \bm{J} \delta\vec{X}
\end{equation}

\begin{itemize}
\item If $\bm{J}$ is invertible, then...
\item If $\bm{J}$ is not invertible and $\bm{J}$ is not zero, them we look for
$$
	\delta\vec{X} = \bm{S} \vec{\lambda}
$$
where the columns of $\bm{S}$ are in $\mathrm{Img\,} \bm{J}$.\\
We also compute $\bm{Z}$ with its   columns   in $\mathrm{Ker\,} J$.\\
So
$$
	\vec{F}(\vec{X}+\delta\vec{X}) \simeq \vec{F}_0 + \bm{J} \bm{S} \vec{\lambda}
$$
and we compute a regularised step
$$
	\delta\vec{X} = -\bm{S}\left(\trn{\bm{S}}\bm{J}\bm{S}\right)^{-1}\trn{\bm{S}}\vec{F} 
$$
with no guarantee that this is a decreasing step.
Let us compute $$\vec{F}_1=\vec{F}(\vec{X}+\delta\vec{X})$$
\end{itemize}




%the full Newton's step is:
%\begin{equation}
%	\vec{p} = - \bm{J}^{-1} \vec{F}
%\end{equation}
%We define
%\begin{equation}
%	g(\lambda) = \dfrac{1}{2} \trn{\vec{F}}  \vec{F} (\vec{X}+\lambda \vec{p})
%\end{equation}
%
%\begin{equation}
%	\vec{\nabla}g = \trn{J}\vec{F}
%\end{equation}
%and we want
%\begin{equation}
%	g(\lambda) \leq g_0 + \alpha \lambda \underbrace{\vec{\nabla}g_0 \cdot \vec{p}}_{-2g_0}
%\end{equation}
%rewritten as
%\begin{equation}
%	g(\lambda) \leq g_0 -\lambda 2 \alpha g_0
%\end{equation}
%
%With a guess $\lambda$:
%\begin{itemize}
%\item if $g(\lambda) \leq g_0 - \lambda 2 \alpha g_0$, accept.
%\item $g(\lambda)\simeq g_0 (1- 2\lambda) + \beta \lambda^2$
%$$\beta = \dfrac{g(\lambda)-g_0(1-2\lambda)}{\lambda^2}$$
%\item $g_0 (1-2\alpha\mu)  =  g_0 (1- 2\mu) + \beta \mu^2$
%$$
%	\mu = \dfrac{2g_0(1-\alpha)}{\beta}
%$$
%\end{itemize}

\end{document}